src/promotion/SimThreadPromotion.v
@@ -30,10 +30,14 @@ Require Import Promotion.
 Require Import SimCommon.
 
 Set Implicit Arguments.
+Set Nested Proofs Allowed.
 
 
 Module SimThreadPromotion.
   Import SimCommon.
+
+
+  (* sim_state *)
 
   Inductive sim_state_synch (l: Loc.t) (r: Reg.t) (st_src st_tgt: State.t): Prop :=
   | sim_state_synch_intro
@@ -49,6 +53,7 @@ Module SimThreadPromotion.
                   (Stmt.instr (Instr.update lhs l (Instr.fetch_add addendum) ordr ordw)) :: stmts_src)
       (STMTS_TGT: st_tgt.(State.stmts) =
                   (Stmt.instr (Instr.assign r (Instr.expr_op2 Op2.add (Value.reg r) addendum))) :: stmts_tgt)
+      (STMTS: stmts_tgt = promote_stmts l r stmts_src)
       (REGS: RegFile.eq_except (RegSet.add lhs (RegSet.singleton r)) st_src.(State.regs) st_tgt.(State.regs))
       (LHS: st_tgt.(State.regs) lhs = st_tgt.(State.regs) r)
   .
@@ -63,6 +68,7 @@ Module SimThreadPromotion.
                   Stmt.instr (Instr.assign lhs (Instr.expr_val (Value.const 1)))
                              :: (Stmt.instr (Instr.assign r new))
                              :: stmts_tgt)
+      (STMTS: stmts_tgt = promote_stmts l r stmts_src)
       (REGS: RegFile.eq_except (RegSet.singleton r) st_src.(State.regs) st_tgt.(State.regs))
       (SUCCESS: st_tgt.(State.regs) r = RegFile.eval_value st_tgt.(State.regs) old)
   .
@@ -75,6 +81,7 @@ Module SimThreadPromotion.
                   (Stmt.instr (Instr.update lhs l (Instr.cas old new) ordr ordw)) :: stmts_src)
       (STMTS_TGT: st_tgt.(State.stmts) =
                   (Stmt.instr (Instr.assign r new)) :: stmts_tgt)
+      (STMTS: stmts_tgt = promote_stmts l r stmts_src)
       (REGS: RegFile.eq_except (RegSet.add lhs (RegSet.singleton r)) st_src.(State.regs) st_tgt.(State.regs))
       (LHS: st_tgt.(State.regs) r = 1)
       (SUCCESS: st_tgt.(State.regs) r = RegFile.eval_value st_tgt.(State.regs) old)
@@ -84,11 +91,12 @@ Module SimThreadPromotion.
   Inductive sim_state_cas_fail (l: Loc.t) (r: Reg.t) (st_src st_tgt: State.t): Prop :=
   | sim_state_cas_fail_intro
       lhs old new ordr ordw stmts_src stmts_tgt
-      (REGS: RegFile.eq_except (RegSet.singleton r) st_src.(State.regs) st_tgt.(State.regs))
       (STMTS_SRC: st_src.(State.stmts) =
                   (Stmt.instr (Instr.update lhs l (Instr.cas old new) ordr ordw)) :: stmts_src)
       (STMTS_TGT: st_tgt.(State.stmts) =
                   Stmt.instr (Instr.assign lhs (Instr.expr_val (Value.const 0))) :: stmts_tgt)
+      (STMTS: stmts_tgt = promote_stmts l r stmts_src)
+      (REGS: RegFile.eq_except (RegSet.singleton r) st_src.(State.regs) st_tgt.(State.regs))
       (FAIL: st_tgt.(State.regs) r <> RegFile.eval_value st_tgt.(State.regs) old)
   .
   Hint Constructors sim_state_cas_fail.
@@ -101,60 +109,140 @@ Module SimThreadPromotion.
     sim_state_cas_fail l r st_src st_tgt
   .
 
-  Inductive sim_thread_promotion (l: Loc.t) (r: Reg.t) (e_src e_tgt: Thread.t lang): Prop :=
-  | sim_thread_promotion_intro
+
+  (* sim_thread *)
+
+  Definition promises_safe (l: Loc.t) (lc: Local.t): Prop :=
+    forall from to val released
+      (GET: Memory.get l to lc.(Local.promises) =
+            Some (from, Message.full val (Some released))),
+      View.le released lc.(Local.tview).(TView.cur).
+
+  Inductive sim_thread (l: Loc.t) (r: Reg.t) (e_src e_tgt: Thread.t lang): Prop :=
+  | sim_thread_intro
       (REGFREE: reg_free_stmts r e_src.(Thread.state).(State.stmts))
-      (STMTS: sim_state l r e_src.(Thread.state) e_tgt.(Thread.state))
+      (STATE: sim_state l r e_src.(Thread.state) e_tgt.(Thread.state))
       (LOCAL: sim_local l e_src.(Thread.local) e_tgt.(Thread.local))
       (SC: sim_timemap l e_src.(Thread.sc) e_tgt.(Thread.sc))
       (MEMORY: sim_memory l e_src.(Thread.memory) e_tgt.(Thread.memory))
+      (FULFILLABLE: fulfillable l e_src.(Thread.local).(Local.tview) e_src.(Thread.memory)
+                                  e_src.(Thread.local).(Local.promises))
       (LATEST: exists from released,
           Memory.get l (Memory.max_ts l e_src.(Thread.memory)) e_src.(Thread.memory) =
           Some (from, Message.full (e_tgt.(Thread.state).(State.regs) r) released))
       (PROMISES: forall to, Memory.get l to e_src.(Thread.local).(Local.promises) = None)
+      (SAFE: promises_safe l e_src.(Thread.local))
   .
-  Hint Constructors sim_thread_promotion.
+  Hint Constructors sim_thread.
 
-  Inductive sim_thread_promotion_reserve (l: Loc.t) (r: Reg.t) (e_src e_tgt: Thread.t lang): Prop :=
-  | sim_thread_promotion_reserve_intro
+  Inductive sim_thread_reserve (l: Loc.t) (r: Reg.t) (e_src e_tgt: Thread.t lang): Prop :=
+  | sim_thread_reserve_intro
       (REGFREE: reg_free_stmts r e_src.(Thread.state).(State.stmts))
-      (STMTS: sim_state l r e_src.(Thread.state) e_tgt.(Thread.state))
+      (STATE: sim_state l r e_src.(Thread.state) e_tgt.(Thread.state))
       (LOCAL: sim_local l e_src.(Thread.local) e_tgt.(Thread.local))
       (SC: sim_timemap l e_src.(Thread.sc) e_tgt.(Thread.sc))
       (MEMORY: sim_memory l e_src.(Thread.memory) e_tgt.(Thread.memory))
-      (LATEST: Memory.latest_val l e_src.(Thread.memory) (e_tgt.(Thread.state).(State.regs) r))
+      (FULFILLABLE: fulfillable l e_src.(Thread.local).(Local.tview) e_src.(Thread.memory)
+                                  e_src.(Thread.local).(Local.promises))
+      (LATEST: exists from from' released,
+          <<MEM: Memory.get l (Memory.max_ts l e_src.(Thread.memory)) e_src.(Thread.memory) =
+                 Some (from, Message.reserve)>> /\
+          <<PROMISE: Memory.get l (Memory.max_ts l e_src.(Thread.memory)) e_src.(Thread.local).(Local.promises) =
+                     Some (from, Message.reserve)>> /\
+          <<LATEST: Memory.get l from e_src.(Thread.memory) =
+                    Some (from', Message.full (e_tgt.(Thread.state).(State.regs) r) released)>>)
       (PROMISES: forall to (TO: to <> Memory.max_ts l e_src.(Thread.memory)),
           Memory.get l to e_src.(Thread.local).(Local.promises) = None)
-      (MEM: exists from,
-          Memory.get l (Memory.max_ts l e_src.(Thread.memory)) e_src.(Thread.memory) =
-          Some (from, Message.reserve))
-      (PROMISE: exists from,
-          Memory.get l (Memory.max_ts l e_src.(Thread.memory)) e_src.(Thread.local).(Local.promises) =
-          Some (from, Message.reserve))
+      (SAFE: promises_safe l e_src.(Thread.local))
   .
-  Hint Constructors sim_thread_promotion_reserve.
+  Hint Constructors sim_thread_reserve.
 
-  (* Lemma step_sim_thread_promotion_reserve *)
-  (*       l r e_src e_tgt *)
-  (*       (SIM: sim_thread_promotion l r e_src e_tgt): *)
-  (*   exists from to e1_src, *)
-  (*     <<STEP: Thread.step false (ThreadEvent.promise l from to Message.reserve Memory.op_kind_add) *)
-  (*                         e_src e1_src>> /\ *)
-  (*     <<SIM: sim_thread_promotion_reserve l r e1_src e_tgt>>. *)
-  (* Proof. *)
-  (*   destruct e_src, e_tgt. inv SIM. ss. *)
-  (*   guardH STMTS. des. *)
-  (* Admitted. *)
 
-  (* Lemma step_sim_thread_promotion *)
-  (*       l r e_src e_tgt *)
-  (*       (SIM: sim_thread_promotion_reserve l r e_src e_tgt): *)
-  (*   exists from to e1_src, *)
-  (*     <<STEP: Thread.step false (ThreadEvent.promise l from to Message.reserve Memory.op_kind_cancel) *)
-  (*                         e_src e1_src>> /\ *)
-  (*     <<SIM: sim_thread_promotion l r e1_src e_tgt>>. *)
-  (* Proof. *)
-  (*   destruct e_src, e_tgt. inv SIM. ss. *)
-  (*   guardH STMTS. des. *)
-  (* Admitted. *)
+  Lemma step_sim_thread_promotion_reserve
+        l r e_src e_tgt
+        (SIM: sim_thread l r e_src e_tgt):
+    exists from to e1_src,
+      <<STEP: Thread.step false (ThreadEvent.promise l from to Message.reserve Memory.op_kind_add)
+                          e_src e1_src>> /\
+      <<SIM: sim_thread_reserve l r e1_src e_tgt>>.
+  Proof.
+    destruct e_src, e_tgt. inv SIM. ss.
+    guardH STATE. des.
+  Admitted.
+
+  Lemma step_sim_thread_promotion
+        l r e_src e_tgt
+        (SIM: sim_thread_reserve l r e_src e_tgt):
+    exists from to e1_src,
+      <<STEP: Thread.step false (ThreadEvent.promise l from to Message.reserve Memory.op_kind_cancel)
+                          e_src e1_src>> /\
+      <<SIM: sim_thread l r e1_src e_tgt>>.
+  Proof.
+    destruct e_src, e_tgt. inv SIM. ss.
+    guardH STATE. des.
+  Admitted.
+
+  Lemma eq_loc_max_ts
+        loc mem1 mem2
+        (EQLOC: forall to, Memory.get loc to mem1 = Memory.get loc to mem2):
+    Memory.max_ts loc mem1 = Memory.max_ts loc mem2.
+  Proof.
+    unfold Memory.max_ts.
+    replace (mem1 loc) with (mem2 loc); ss.
+    apply Cell.ext. eauto.
+  Qed.
+
+  Lemma sim_thread_promise_step
+        l r e1_src
+        pf e_tgt e1_tgt e2_tgt
+        (SIM1: sim_thread l r e1_src e1_tgt)
+        (WF1_SRC: Local.wf e1_src.(Thread.local) e1_src.(Thread.memory))
+        (WF1_TGT: Local.wf e1_tgt.(Thread.local) e1_tgt.(Thread.memory))
+        (CLOSED1_SRC: Memory.closed e1_src.(Thread.memory))
+        (STEP_TGT: Thread.promise_step pf e_tgt e1_tgt e2_tgt):
+    exists e_src e2_src,
+      <<STEP_SRC: Thread.opt_promise_step e_src e1_src e2_src>> /\
+      <<SIM2: sim_thread l r e2_src e2_tgt>>.
+  Proof.
+    inversion STEP_TGT. subst.
+    destruct (Loc.eq_dec loc l).
+    { subst. inv LOCAL; ss.
+      esplits; [econs 1|]; eauto.
+      inv SIM1. ss.
+      exploit promise_loc; try exact PROMISE; try apply LOCAL; eauto. i. des.
+      econs; ss; eauto.
+      econs; ss; eauto; try apply LOCAL.
+    }
+    exploit promise_step; try exact LOCAL; try apply SIM1;
+      try apply WF1_SRC; try apply WF1_TGT; eauto.
+    i. des.
+    destruct e1_src. ss.
+    esplits.
+    - econs 2. econs; eauto.
+    - inv SIM1. inv STEP_SRC. ss.
+      econs; eauto; ss; ii.
+      + erewrite <- promise_eq_mem; eauto.
+        erewrite <- eq_loc_max_ts; eauto.
+        eapply promise_eq_mem; eauto.
+      + erewrite <- promise_eq_promises; eauto.
+      + erewrite <- promise_eq_promises in GET; eauto.
+  Qed.
+
+  Lemma sim_thread_program_step
+        l r e1_src
+        e_tgt e1_tgt e2_tgt
+        (SIM1: sim_thread l r e1_src e1_tgt)
+        (WF1_SRC: Local.wf e1_src.(Thread.local) e1_src.(Thread.memory))
+        (WF1_TGT: Local.wf e1_tgt.(Thread.local) e1_tgt.(Thread.memory))
+        (SC1_SRC: Memory.closed_timemap e1_src.(Thread.sc) e1_src.(Thread.memory))
+        (SC1_TGT: Memory.closed_timemap e1_tgt.(Thread.sc) e1_tgt.(Thread.memory))
+        (CLOSED1_SRC: Memory.closed e1_src.(Thread.memory))
+        (CLOSED1_TGT: Memory.closed e1_tgt.(Thread.memory))
+        (STEP_TGT: Thread.program_step e_tgt e1_tgt e2_tgt):
+    exists e_src e1_src e2_src,
+      <<STEP_SRC: Thread.opt_program_step e_src e1_src e2_src>> /\
+      <<EVENT: ThreadEvent.get_machine_event e_src = ThreadEvent.get_machine_event e_tgt>> /\
+      <<SIM2: sim_thread l r e2_src e2_tgt>>.
+  Proof.
+  Admitted.
 End SimThreadPromotion.
